moved to sigmaType-characterisation of restricted problems

theories/L/Complexity/NP.v
@@ -20,30 +20,30 @@ Section NP_certificate_fix.
   Definition polyBalanced R :Prop :=
     exists f, inOPoly f /\ (forall x y, R x y -> size (enc y) <= f (size (enc x))) /\ monotonic f.
 
-  Definition inTimePoly {X} `{registered X} P:=
+  Definition inTimePoly {X} `{registered X} `(P:restrictedP vX):=
     exists f, decInTime P f /\ inOPoly f /\ monotonic f.
 
 
 End NP_certificate_fix.
 
 Local Set Warnings "-cannot-define-projection".
-Record inNP {X} `{registered X} (P:restrictedP X) : Prop :=
+Record inNP {X} `{registered X} `(P:restrictedP (X:=X) vX) : Prop :=
   inNP_introSpec
     {
       (*Y : Type;
     reg__Y : registered Y;*)
       R : X -> term -> Prop; (* fixed to term for simplicity *)
-      poly__R : inTimePoly (fun '(x,y) => (fst (P x), R x y));
-      bal__R : polyBalanced R;
-      spec__R : forall x, fst (P x) -> snd (P x) <-> exists y, R x y
+      poly__R : inTimePoly (vX:= fun '(x,_) => vX x) (fun '(exist _ (x,y) Hx) => (R x y));
+      bal__R : polyBalanced R; (*TODO: What if moved to spec__R(better: move condition externally)? and only require that some small certificate satisfies condition? It seems that we might want that every certificate is valid, but there must exist a small one? *)
+      spec__R : forall x Hx, P (exist _ x Hx) <-> exists y, R x y
     }.
 
 
-Lemma inNP_intro {X Y} `{_:registered X} `{registered Y} {_:decodable Y} (P:restrictedP X) (R:X -> Y -> Prop):
+Lemma inNP_intro {X Y} `{_:registered X} `{registered Y} {_:decodable Y} `(P:@restrictedP X vX) (R:X -> Y -> Prop):
   polyTimeComputable (decode Y)
-  -> inTimePoly (fun '(x,y) => (fst (P x), R x y))
+  -> inTimePoly (vX:= fun '(x,_) => vX x) (fun '(exist _ (x,y) Hx) => (R x y))
   -> polyBalanced R
-  ->  ( forall x, fst (P x) -> snd(P x) <-> exists y, R x y)
+  ->  (forall x Hx, P (exist _ x Hx) <-> exists y, R x y)
   -> inNP P.
 Proof.
   intros decode__comp poly_R bal_R spec_R.
@@ -78,12 +78,12 @@ Proof.
        unfold t__f';reflexivity.
       *rewrite polyTimeC__mono with (x':=(size (enc a) + size (enc b) + 4)). 2:lia.
        unfold t__f'. lia.
-     +unfold f'. intros []. cbn.
-      destruct decode eqn:H'.
-      *etransitivity. 2:now apply decInTime_correct. cbn iota beta.
+     +unfold f'. intros [x] Hx. cbn.
+      destruct decode  as [y| ] eqn:H'.
+      *etransitivity. 2:eapply decInTime_correct. 2:eauto.
        eapply decode_correct2 in H'. symmetry in H'.
-       split;[intros (?&?&?)|intros ?].
-       --cbn [snd]. enough (x0 = y) by congruence. eapply inj_enc.  rewrite <- H', <- H3. reflexivity.
+       split;[intros (y'&?&?)|intros ?].
+       --enough (y = y') by congruence. eapply inj_enc. congruence.
        --eauto.
       *split.  2:eauto.
        intros (?&->&?). rewrite decode_correct in H'.  easy.
@@ -94,31 +94,30 @@ Qed.
 
 (** ** Poly Time Reduction s*)
 
-
-Record reducesPolyMO X Y `{registered X} `{registered Y} (P : restrictedP X) (Q : restrictedP Y) :Prop :=
-  reducesPolyMO_introSpec {
+Generalizable Variable vY.
+Record reducesPolyMO X Y `{registered X} `{registered Y} `(P : restrictedP vX) `(Q : restrictedP vY) :Prop :=
+  reducesPolyMO_intro {
       f : X -> Y;
       f__comp : polyTimeComputable f;
-      f__correct : forall x, fst (P x) -> (snd (P x) <-> snd (Q (f x)));
-      f__correctRestr : forall x, fst (P x) -> fst (Q (f x))
+      f__correct : (forall x (Hx : vX x), {Hy : vY (f x) & (P (exist _ x Hx)) <-> (Q (exist _ (f x) Hy))})
     }.
 
 Notation "P ⪯p Q" := (reducesPolyMO P Q) (at level 50).
 
-Lemma reducesPolyMO_intro X Y `{RX: registered X} `{RY:registered Y} (P : restrictedP X) (Q : restrictedP Y) f:
+(*
+Lemma reducesPolyMO_intro X Y `{RX: registered X} `{RY:registered Y} `(P : restrictedP vX) `(Q : restrictedP vY) f:
   polyTimeComputable f
-  -> (forall x, fst (P x) -> fst (Q (f x)) /\ (snd (P x) <-> snd (Q (f x))))
+  -> (forall x (Hx : vX x), {Hy : vY (f x) & (P (exist _ x Hx)) <-> (Q (exist _ (f x) Hy))})
   -> P ⪯p Q.
 Proof.
-  intros H H'. econstructor. eassumption. all:intros ? ?. all:now eapply H'.
-Qed.
+  intros H H'. econstructor. eassumption. all:intros ? ?. all:try now eapply H'.
+Qed. *)
 
-Lemma reducesPolyMO_restriction_antimonotone X `{R :registered X} (P Q:restrictedP X) :
-    (forall x, fst (P x) -> fst (Q x))
-    -> (forall x, fst (P x) -> snd (P x) <-> snd (Q x))
-    -> P ⪯p Q.
+Lemma reducesPolyMO_restriction_antimonotone X `{R :registered X} {vP} (P:restrictedP vP) {vQ} (Q:restrictedP vQ):
+  (forall (x : X) HvP, {HvQ : vQ x & P (exist vP x HvP) <-> Q (exist vQ x HvQ)})
+  -> P ⪯p Q.
 Proof.
-  exists (fun x => x). 2,3:easy.
+  exists (fun x => x). 2:now eauto. 
   exists (fun _ => 1).
   -constructor. extract. solverec.
   -smpl_inO.
@@ -126,18 +125,21 @@ Proof.
   -exists (fun x => x). repeat split. 2-3:now smpl_inO.  reflexivity.
 Qed.
 
-Lemma reducesPolyMO_reflexive X {regX : registered X} P : P ⪯p P.
+Lemma reducesPolyMO_reflexive X {regX : registered X} `(P : restrictedP vX) : P ⪯p P.
 Proof.
-  apply reducesPolyMO_restriction_antimonotone. all:easy. 
+  eapply reducesPolyMO_restriction_antimonotone. esplit. reflexivity. 
 Qed.
 
-Lemma reducesPolyMO_transitive X Y Z {regX : registered X} {regY : registered Y} {regZ : registered Z} (P : restrictedP X) (Q : restrictedP Y) (R : restrictedP Z) :
+Lemma reducesPolyMO_transitive X Y Z {vX vY vZ} {regX : registered X} {regY : registered Y} {regZ : registered Z} (P : restrictedP (X:=X)vX) (Q : restrictedP (X:=Y)vY) (R : restrictedP (X:=Z)vZ) :
   P ⪯p Q -> Q ⪯p R -> P ⪯p R.
 Proof.
-  intros [f Cf Hf Hf'] [g Cg Hg Hg'].
+  intros [f Cf Hf] [g Cg Hg].
   exists (fun x =>g (f x)).
-  2:now intros; rewrite Hf,Hg.
-  2:easy. 
+  2:{intros ? ?;clear - Hf Hg.
+     edestruct Hf as (Hfx&Hf').
+     edestruct Hg as (Hgfx&Hg'). eexists. rewrite Hf',Hg'. reflexivity.
+  }
+  clear Hf Hg.
   destruct Cf as [t__f [] ? f__mono (sizef&H__sizef&?&?)], Cg as [t__g [] ? g__mono (size__g&?&?&?)].
   exists (fun x => t__f x + t__g (sizef x) + 1).
   -split. extract. solverec.
@@ -152,7 +154,7 @@ Proof.
    +eapply monotonic_comp. all:try eassumption.
 Qed.
 
-Lemma red_inNP X Y `{regX : registered X} `{regY : registered Y} (P : restrictedP X) (Q : restrictedP Y) :
+Lemma red_inNP X Y `{regX : registered X} `{regY : registered Y} `(P : restrictedP (X:=X) vX) `(Q : restrictedP (X:=Y) vY) :
   P ⪯p Q -> inNP Q -> inNP P.
 Proof.
   intros [f Cf Hf] [R polyR bal specR].
@@ -170,8 +172,7 @@ Proof.
      erewrite mono_f'__t with (x':=_). reflexivity.
      rewrite H__fs.
      rewrite mono__fs with (x':=(size (enc a) + size (enc b) + 4)). all:Lia.nia.
-    *intros [x z] ?. rewrite <- H__f'.
-     all:cbn. all:easy. 
+    *intros [x c] Hx. destruct (Hf _ Hx) as [Hfx _]. apply H__f' with (x:=(f x,c)). easy. 
    +split.
     all:smpl_inO.
     { eapply inOPoly_comp. all:smpl_inO. }
@@ -184,35 +185,45 @@ Proof.
     hnf in Hf__mono.
     rewrite Hf__mono. 2:eapply H__fs. reflexivity.
    +eapply monotonic_comp. all:eassumption.
-  -intros x ?.
-   rewrite Hf. apply specR. all:easy. 
+  -intros x Hx.
+   specialize (Hf _ Hx) as (?&Hf). rewrite Hf. apply specR. 
 Qed.
 
 
 
 
 (** ** NP Hardness and Completeness *)
-Definition NPhard X `{registered X} P :=
-  forall Y `{registeredP Y} Q,
+Definition NPhard X `{registered X} `(P:restrictedP vX) :=
+  forall Y `{registeredP Y} vY (Q:restrictedP (X:=Y) vY),
     inNP Q -> Q ⪯p P.
 
-Lemma red_NPhard X Y `{registered X} `{registered Y} (P:restrictedP X) (Q:restrictedP Y)
+Lemma red_NPhard X Y `{registered X} `{registered Y} `(P:restrictedP (X:=X) vX) `(Q:restrictedP (X:=Y) vY)
   : P ⪯p Q -> NPhard P -> NPhard Q.
 Proof.
   intros R hard.
-  intros ? ? ? Q' H'. apply hard in H'.
-  eapply reducesPolyMO_transitive with (1:=H'). all:eassumption.
+  intros ? ? ? ? Q' H'. apply hard in H'. 2:easy. 
+  eapply reducesPolyMO_transitive  with (1:=H'). all:eassumption.
 Qed.
 
-Corollary NPhard_traditional X `{registered X} P:
-  NPhard P -> NPhard (unrestrictedP (fun x => snd (P x))).
+Corollary NPhard_traditional X `{registered X} vX `(P : X -> Prop):
+  NPhard (fun (x:{x | vX x}) => P (proj1_sig x)) -> NPhard (unrestrictedP P).
 Proof.
   eapply red_NPhard.
   eapply reducesPolyMO_restriction_antimonotone.
   all: cbn. all:easy.
 Qed.
 
-Definition NPcomplete X `{registered X} P :=
+Corollary NPhard_traditional2 X `{registered X} `{Pv : restrictedP vX} (P : X -> Prop):
+  (forall (x : X) (Hv : vX x), Pv (exist vX x Hv) <-> P x)
+  -> NPhard Pv -> NPhard (unrestrictedP P).
+Proof.
+  intros H'.
+  eapply red_NPhard.
+  eapply reducesPolyMO_restriction_antimonotone.
+  all: cbn. all:easy.
+Qed.
+
+Definition NPcomplete X `{registered X} `(P : restrictedP vX) :=
   NPhard P /\ inNP P.
 
 Hint Unfold NPcomplete.
